One_step is completed. Only left is extension functions.

src/SmallCoreAlg.v
@@ -31,11 +31,64 @@ Theorem typing_alg_progress:
     intros. eapply progress. eapply typing_alg_leg; eauto.
 Qed.
 
-Fixpoint progress' (t: tm) : tm.
+Theorem eq_extty_dec:
+    forall (X Y : Extty),
+        {X = Y} + {X <> Y}.
+    
+    intros X.
+    induction X; intro Y;
+    induction Y; intros; subst; eauto;
+    try (
+        left; eauto; fail);
+    try (
+        right; intro; 
+        try match goal with
+        | h : _ = _ |- _ => inversion h; subst; eauto; try discriminate
+        end; eauto; try discriminate; fail
+    ).
+    destruct (eq_id_dec t t0); subst; eauto;
+    try (
+        left; eauto; fail);
+    try (
+        right; intro; 
+        try match goal with
+        | h : _ = _ |- _ => inversion h; subst; eauto; try discriminate
+        end; eauto; try discriminate; fail
+    ).
+
+    destruct (eq_id_dec t t0); subst; eauto.
+    clear IHY.
+    destruct (IHX Y); destructALL; subst; eauto;
+    try (
+        left;subst; eauto; fail);
+    try (
+        right; intro; 
+        try match goal with
+        | h : _ = _ |- _ => inversion h; subst; eauto; try discriminate
+        end; eauto; try discriminate; fail
+    ).
+    right; intro. inversion H; subst; eauto.
+
+    clear IHY1; clear IHY2.
+    destruct (IHX1 Y1); destruct (IHX2 Y2); destructALL;
+    try (
+        left; subst; eauto; fail);
+    try (
+        right; intro; 
+        try match goal with
+        | h : _ = _ |- _ => inversion h; subst; eauto; try discriminate
+        end; eauto; try discriminate; fail
+    ).
+Qed.
+
+
+
+
+Fixpoint one_step (t: tm) : tm.
     refine (
         match t with
         | tapp f x => _
-        | tlet i T h bind body => subst i bind body
+        | tlet i T h bind body => _
         | tfixApp i T h self => subst i (tfixApp i T h self) self 
         | tleft lt RT h => _
         | tright LT h rt => _
@@ -47,25 +100,182 @@ Fixpoint progress' (t: tm) : tm.
 
     (* case tapp *)
     destruct (value_dec f);
-    destruct (value_dec x).
+    try (
+        match goal with
+        | h : ~value ?F |- _=> exact (tapp (one_step F) x)
+        end
+    );
+    destruct (value_dec x);
+    try (
+        match goal with
+        | h : ~value ?X |- _=> exact (tapp f (one_step x))
+        end
+    ).
+
 
     destruct f eqn:h0;
     (
         match goal with
-        | h: f = (tfun _ _)
-    )
+        | h: f = (tfun _ _ _ _) |- _ => idtac
+        | h: f = (tfield _ _ _ _) |- _ => idtac
+        | h : f = text _ _ _ |- _ => idtac
+        | |- _ => exact t
+        end
+    ).
 
+    (* case f = tfun *)
+    exact (subst i x t1).
+    (* case f = text *)
+        destruct x eqn: h1;
+        match goal with
+        | h : x = text _ _ _ |- _ => idtac
+        | |- _ => exact t
+        end.
+        destruct T eqn: h2;
+        match goal with
+        | h : T = ETFun _ _ |- _ => idtac
+        | |- _ => exact t
+        end.
+        destruct (eq_extty_dec (ETVar t3) T0).
+        subst.
+        destruct (ExttmInterpreter t3 e1 t1 t2 e e0).
+        exact (text e1 x e2).
+        exact t.
+    (* case f = tfield *)
+    destruct (rcd_field_tm' x i) eqn:h2.
+    exact t1.
+    exact t.
+    (* case tlet *)
+    destruct (value_dec bind).
 
+    exact (subst i bind body).
+    exact (tlet i T h (one_step bind) body).
+
+    (* case tleft*)
+    destruct (value_dec lt).
+    exact t.
+    exact (tleft (one_step lt) RT h).
+
+    (* case tright *)
+    destruct (value_dec rt).
+    exact t.
+    exact (tright LT h (one_step rt)).
+
+    (* case tcase *)
+
+    destruct (value_dec crit);
+    try (
+        match goal with
+        | h : ~value crit |- _ => exact (tcase (one_step crit) lb rb)
+        end
+    ).
+    destruct (value_dec lb);
+    try (
+        match goal with
+        | h : ~value lb |- _ => exact (tcase crit (one_step lb) rb)
+        end
+    ).
+    destruct (value_dec rb);
+    try (
+        match goal with
+        | h : ~value rb |- _ => exact (tcase crit lb (one_step rb))
+        end
+    ).
+    destruct crit eqn:h0;
+    match goal with
+    | h : crit = tleft ?t _ _ |- _ => exact (tapp lb t)
+    | h : crit = tright _ _ ?t |- _ => exact (tapp rb t)
+    | h : crit = text _ _ _ |- _ => idtac
+    | |- _ => exact t
+    end.
+    destruct T eqn: h1;
+    match goal with
+    | h : T = ETSum _ _ |- _ => idtac
+    | |- _ => exact t
+    end.
+    destruct (ExttmSumResolver e0_1 e0_2 t1 e) eqn:h2.
+    destruct s. exact (tapp lb (text e0_1 x e0)).
+    destruct s. exact (tapp rb (text e0_2 x e0)).
+
+    destruct (value_dec head);
+    try (
+        match goal with
+        | h : ~value head |- _ => exact (trcons i (one_step head) tail)
+        end
+    ).
+    destruct (value_dec tail);
+    try (
+        match goal with
+        | h : ~value tail |- _ => exact (trcons i head (one_step tail))
+        end
+    ).
+    exact t.
+Defined.
+
+Theorem one_step_value_id:
+    forall x,
+        value x ->
+        one_step x = x.
+
+    intros x; induction x;
+    intros; subst; cbn in *; eauto; try discriminate;
+    repeat (
+        match goal with
+        | |- (if ?x then _ else _) = _ => 
+            let c := fresh c in
+                destruct x eqn:c; try contradiction; try discriminate; eauto
+        | h : value (_ _) |- _ => inversion h; subst; eauto;try contradiction; try discriminate; clear h
+
+        end
+    ).
+Qed.
+
+Axiom eq_is_only_eq:
+    forall (X:Set) (x: X) (y: x = x), y = eq_refl.
+
+Theorem one_step_step:
+    forall t t',
+        step t t' ->
+        one_step t = t'.
+
+    intros t t' h.
+    induction h; intros; subst; cbn in *; eauto; try discriminate;
+    repeat (
+        match goal with
+        | |- (if ?x then _ else _) = _ => 
+            let c := fresh c in
+                destruct x eqn:c; try contradiction; try discriminate; eauto
+        | |- (match ?x with _ => _ end) = _ =>
+            let c := fresh c in
+            destruct x eqn:c; try contradiction; try discriminate; eauto
+        | |- (match ?x with _ => _ end) _ = _ =>
+            let c := fresh c in
+            destruct x eqn:c; try contradiction; try discriminate; eauto
+        | h : value (_ _) |- _ => inversion h; subst; eauto;try contradiction; try discriminate; clear h
+        end
+    );
+    try tac_value_no_step;
+    try (
+        match goal with
+        | h : ~ (value (?x)) |- _ =>
+            assert (value x); eauto
+        end; try contradiction
+    ).
+
+    (* case tcase *)
+    inversion H1; subst; eauto.
+    rewrite (Exteqeq _ _ e h'); eauto.
+    inversion H1; subst; eauto.
+    rewrite (Exteqeq _ _ e h'); eauto.
+    (* case tfield *)
+    inversion H0; subst; eauto.
+
+    (* case tapp *)
     
-
-
-Definition one_step_interpret (t : tm) : option tm.
-    destruct (check_type empty t) eqn:h0;
-    NotNoneInCtx.
-
-    forwards*: typing_alg_leg.
-    forwards*: progress.
-    destruct H0.
+    compute. 
+    rewrite (eq_is_only_eq _ _ e).
+    destruct (eintp i O f x h0 h1). eauto.
+Qed.
 
 
 
